Updated files Lab4

labclasses/lab4/lab4.dfy
@@ -5,6 +5,23 @@
  * array, and the position at which the new element was inserted.
  */
 
-method sortedInsertion(a:array<int>, na:int, e:int) returns (z:array<int>,
-nz:int, pos:int)
-{}
+method sortedInsertion(a:array<int>, na:int, e:int) returns (z:array<int>, nz:int, pos:int)
+{
+
+}
+
+function sortedRange(a:array<char>, l:int, h:int):bool
+    requires 0 <= l <= h <= a.Length
+    reads a
+{ forall i, j:: (l <= i < j < h) ==> a[i] <= a[j] }
+
+function sorted(a:array<char>, n:int):bool
+    requires 0 <= n <= a.Length
+    reads a
+{ forall i, j:: (0 <= i < j < n) ==> a[i] <= a[j] }
+
+method insert(a:array<char>, i:int, v:char, n:int)
+  requires 0 <= n < a.Length
+  requires sorted(a, n)
+  modifies a 
+  ensures sorted(a, n+1)
